exam_e8.v
@@ -1,0 +1,78 @@
+Require Import String.
+Require Import List.
+Require Import Arith.
+Require Import Arith.Compare.
+Import ListNotations.
+Require Import TacticsL8.
+
+Inductive RoboLang : Type :=
+| Skip
+| MoveRight (n: nat)
+| MoveLeft (n: nat)
+| Pick
+| Drop
+| Seq (e1 e2: RoboLang).
+
+Fixpoint replace {X:Type} (n: nat) (l: list X) (x:X) : list X :=
+match n, l with
+| 0   , h :: t => x :: t
+| _   , []     => []
+| S n', h :: t => h :: (replace n' t x)
+end.
+
+Fixpoint eval (e: RoboLang) (st: ((nat*(option string))*(list (option string))))
+                               : ((nat*(option string))*(list (option string))) :=
+match st with
+| ((pos, hold), env) => match e with
+                        | Skip        => st
+                        | MoveRight n => ((pos+n, hold), env)
+                        | MoveLeft n  => if negb ((pos-1) <? 0) then
+                                           ((pos-n, hold), env)
+                                         else
+                                           ((0, hold), env)
+                        | Pick        => match hold with
+                                         | None => ((pos, (nth pos env None)), (replace pos env None))
+                                         | Some s => st
+                                         end
+                        | Drop        => match (nth pos env None) with
+                                         | None => ((pos, None), (replace pos env hold))
+                                         | Some s => st
+                                         end
+                        | Seq e1 e2   => eval e2 (eval e1 st)
+                        end
+end.
+
+Theorem natPnMn : forall n, n - n = 0.
+Proof.
+  intros. induction n.
+  - easy.
+  - simpl. rewrite IHn. easy.
+Qed.
+
+Theorem natAPnMn : forall a n, a + n - n = a.
+Proof.
+  intros. cut ((n-n) = 0).
+  - intros. induction a.
+    + simpl. exact H.
+    + rewrite <- IHa at 2. linear_arithmetic.
+  - apply natPnMn.
+Qed.
+
+Theorem mvNRNL : forall n st, (eval (Seq (MoveRight n) (MoveLeft n)) st) = st.
+Proof.
+  intros. induction st. induction a. rename a into pos. rename b0 into hold. rename b into env.
+  simpl. cut ((pos + n - n) = pos).
+    + intros. rewrite H. easy.
+    + apply natAPnMn.
+Qed.
+
+Fixpoint opt1 (e: RoboLang) : RoboLang :=
+match e with
+| Seq (MoveRight a) (MoveLeft b) => if beq_nat a b then Skip else Seq (MoveRight a) (MoveLeft b)
+| Skip => Skip
+| MoveRight n => MoveRight n
+| MoveLeft n => MoveLeft n
+| Pick => Pick
+| Drop => Drop
+| Seq a b => Seq (opt1 a) (opt1 b)
+end.
